Example of rewriting a function. Fixed quotation section.

doc/ExampleInspect.fst
@@ -9,3 +9,14 @@ let show_an_arrow_expr () : Tac unit =
      exact t
 
 let addition : int -> int -> int = synth_by_tactic show_an_arrow_expr
+
+let show_term _ : Tac unit = 
+  let t = (`(fun (z:int) -> z)) in
+    print (term_to_ast_string t);
+  let t2 = (`(fun (z:int{z<2}) -> z)) in
+    print (term_to_ast_string t2);
+  exact (quote 1)
+
+let foo : int = synth_by_tactic show_term
+
+
