doc/ExampleRewrite.fst
@@ -1,0 +1,34 @@
+module ExampleRewrite
+
+open FStar.Tactics
+
+// Match fun x -> <constant integer>
+let match_constant (t:term) : Tac int =
+  match inspect t with
+  | Tv_Abs binder body -> 
+     ( print ("binder: " ^ (binder_to_string binder));
+       print ("body: " ^ (term_to_ast_string body));
+       match body with 
+     | Tv_Const (C_Int v) -> v
+     | _ -> fail "not an integer constant"
+     )
+  | _ -> fail "not an abtraction"
+                 
+val rewrite_constant : (int->int)  -> Tac unit
+let rewrite_constant f = 
+  let t1 = (quote f) in
+    print ("original term: " ^ (term_to_ast_string t1));
+    let t2 = norm_term_env (top_env()) [delta] t1 in
+      print ("after delta: " ^ (term_to_ast_string t2));    
+      let orig_int = match_constant t2 in
+        (exact (quote (fun x -> (op_Multiply orig_int 2))))
+
+
+let a (x:int) : int = 5
+
+let foo: int->int = synth_by_tactic (fun () -> rewrite_constant a)
+
+let _ = assert( foo 3 = 10 )
+
+    
+  
